Mitigate more

backend/RTLgenproof.v
@@ -27,6 +27,31 @@ Require Import sflib.
   distinct pseudo-registers.
 *)
 
+Section LEX_ORDER.
+
+Context {A B: Type}.
+Variable ordA: A -> A -> Prop.
+Variable ordB: B -> B -> Prop.
+
+Inductive lex_ord: A*B -> A*B -> Prop :=
+  | lex_ord_left: forall a1 b1 a2 b2,
+      ordA a1 a2 -> lex_ord (a1, b1) (a2, b2)
+  | lex_ord_right: forall a b1 b2,
+      ordB b1 b2 -> lex_ord (a, b1) (a, b2).
+
+Lemma wf_lex_ord:
+  well_founded ordA -> well_founded ordB -> well_founded lex_ord.
+Proof.
+  intros Awf Bwf.
+  assert (forall a, Acc ordA a -> forall b, Acc ordB b -> Acc lex_ord (a, b)).
+    induction 1. induction 1. constructor; intros. inv H3.
+    apply H0. auto. apply Bwf.
+    apply H2; auto.
+  red; intros. destruct a as [a b]. apply H; auto.
+Qed.
+
+End LEX_ORDER.
+
 Record map_wf (m: mapping) : Prop :=
   mk_map_wf {
     map_wf_inj:
@@ -1118,8 +1143,8 @@ Fixpoint size_cont (k: cont) : nat :=
 
 Definition measure_state (S: CminorSel.state) :=
   match S with
-  | CminorSel.State _ s k _ _ _ => (ppair (size_stmt s + size_cont k) (size_stmt s))
-  | _                           => (ppair 0 0)
+  | CminorSel.State _ s k _ _ _ => ((size_stmt s + size_cont k), (size_stmt s))
+  | _                           => (0, 0)
   end.
 
 Definition lt_state (S1 S2: CminorSel.state) :=
